theories/ExprProp.v
@@ -1,5 +1,4 @@
 Require Import Coq.Lists.List.
-Require Import MirrorCore.Iso.
 Require Import MirrorCore.TypesI.
 Require Import MirrorCore.ExprI.
 
@@ -7,20 +6,20 @@ Set Implicit Arguments.
 Set Strict Implicit.
 
 Section semantic.
-  Variable typ : Type.
-  Variable typD : list Type -> typ -> Type.
-  Context {RType_typ : RType typD}.
-  Variable TI_prop : TypInstance0 typD Prop.
+  Context {RType_typ : RType}.
+  Variable TI_prop : Typ0 _ Prop.
   Variable expr : Type.
-  Context {Expr_expr : Expr typD expr}.
+  Context {Expr_expr : Expr _ expr}.
 
-  Let tvProp := @typ0 _ _ _ TI_prop.
+  Let tvProp := @typ0 _ _ TI_prop.
 
   Definition Provable_val (val : typD nil tvProp) : Prop :=
-    @soutof _ _ (@typ0_iso _ _ _ TI_prop nil) (fun x => x) val.
+    match typ0_cast nil in _ = t return t with
+      | eq_refl => val
+    end.
 
   Definition Provable uvars vars (e : expr) : Prop :=
-    match exprD (typD := typD) uvars vars e tvProp with
+    match exprD uvars vars e tvProp with
       | None => False
       | Some p => Provable_val p
     end.
@@ -29,28 +28,3 @@ Section semantic.
     Forall (Provable uvars vars) es.
 
 End semantic.
-
-(*
-Theorem AllProvable_weaken : forall ts (fs : functions ts) u ue v ve es,
-  AllProvable fs u v es -> AllProvable fs (u ++ ue) (v ++ ve) es.
-Proof.
-  induction 1; constructor; eauto.
-  { unfold Provable in *. destruct H.
-    eapply exprD_weaken in H. destruct H. intuition. eauto. }
-Qed.
-
-Theorem Forall_cons : forall T (P : T -> Prop) x xs,
-  Forall P (x :: xs) <-> P x /\ Forall P xs.
-Proof.
-  intuition; inversion H; auto.
-Qed.
-
-Theorem AllProvable_app : forall ts (fs : functions ts) u v es es',
-  AllProvable fs u v (es ++ es') <-> AllProvable fs u v es /\ AllProvable fs u v es'.
-Proof.
-  unfold AllProvable.
-  induction es; simpl; intros.
-  { intuition. }
-  { repeat rewrite Forall_cons. rewrite IHes. intuition. }
-Qed.
-*)
